crefine + infoflowc: adjust proofs for new Haskell assertion
The new kernelExitAssertions need to be threaded through the fastpath
and integrated in the right place in the theorems about callKernel.

In InfoFlowC we have yet another refinement framework, and we're taking apart
callKernel to isolate the `schedule` call which is significant in the
infoflow proof and needs the new assertion inserted as wel. After some force
applied, this does work as well.

Signed-off-by: Gerwin Klein <gerwin.klein@data61.csiro.au>

proof/infoflow/ADT_IF_Refine.thy
@@ -10,13 +10,15 @@ begin
 
 context begin interpretation Arch . (*FIXME: arch_split*)
 
-definition
-  kernelEntry_if
-where
+definition kernelEntry_if where
   "kernelEntry_if e tc \<equiv> do
     t \<leftarrow> getCurThread;
     threadSet (tcbArch_update (atcbContextSet tc)) t;
     r \<leftarrow> handleEvent e;
+    stateAssert (\<lambda>s. valid_domain_list' s \<and>
+                     (e \<noteq> Interrupt \<longrightarrow> 0 < ksDomainTime s) \<and>
+                     (e = Interrupt \<longrightarrow> ksDomainTime s = 0 \<longrightarrow>
+                       ksSchedulerAction s = ChooseNewThread)) [];
     return (r,tc)
   od"
 
@@ -26,7 +28,8 @@ definition prod_lift where "prod_lift R r r' \<equiv> R (fst r) (fst r') \<and> 
 
 lemma kernel_entry_if_corres:
   "corres (prod_lift (intr \<oplus> dc)) (einvs and (\<lambda>s. event \<noteq> Interrupt \<longrightarrow> ct_running s) and
-                       (\<lambda>s. scheduler_action s = resume_cur_thread))
+                       (\<lambda>s. scheduler_action s = resume_cur_thread) and
+                       (\<lambda>s. 0 < domain_time s) and valid_domain_list)
                       (invs' and (\<lambda>s. event \<noteq> Interrupt \<longrightarrow> ct_running' s) and
                        (\<lambda>s. vs_valid_duplicates' (ksPSpace s)) and
                        (\<lambda>s. ksSchedulerAction s = ResumeCurrentThread))
@@ -46,10 +49,18 @@ lemma kernel_entry_if_corres:
           apply (clarsimp simp: tcb_cte_cases_def)
          apply (simp add: exst_same_def)
         apply (rule corres_split [OF _ he_corres])
-          apply (clarsimp simp: prod_lift_def)
-         apply (wp  hoare_TrueI threadSet_invs_trivial thread_set_invs_trivial
-                   thread_set_not_state_valid_sched thread_set_ct_running threadSet_ct_running' static_imp_wp
-               | simp add: tcb_cap_cases_def)+
+          apply (rule corres_stateAssert_assume_stronger[where Q=\<top> and
+                        P="\<lambda>s. valid_domain_list s \<and>
+                               (event \<noteq> Interrupt \<longrightarrow> 0 < domain_time s) \<and>
+                               (event = Interrupt \<longrightarrow> domain_time s = 0 \<longrightarrow>
+                                 scheduler_action s = choose_new_thread)"])
+           apply (clarsimp simp: prod_lift_def)
+          apply (clarsimp simp: state_relation_def)
+         apply (wp hoare_TrueI threadSet_invs_trivial thread_set_invs_trivial
+                   thread_set_not_state_valid_sched thread_set_ct_running threadSet_ct_running'
+                   hoare_vcg_const_imp_lift handle_event_domain_time_inv
+                   handle_interrupt_valid_domain_time
+               | simp add: tcb_cap_cases_def | wpc | wp (once) hoare_drop_imps)+
    apply (force simp: invs_def cur_tcb_def)
   apply force
   done
@@ -61,6 +72,7 @@ lemma kernelEntry_invs'[wp]:
     kernelEntry_if e tc \<lbrace>\<lambda>_. invs'\<rbrace>"
   apply (simp add: kernelEntry_if_def)
   apply (wp threadSet_invs_trivial threadSet_ct_running' static_imp_wp
+         | wp (once) hoare_drop_imps
          | clarsimp)+
   done
 
@@ -72,6 +84,7 @@ lemma kernelEntry_valid_duplicates[wp]:
   apply (simp add: kernelEntry_if_def)
   apply (wp handleEvent_valid_duplicates'
             threadSet_invs_trivial threadSet_ct_running' static_imp_wp
+         | wp (once) hoare_drop_imps
          | clarsimp)+
   done
 
@@ -113,7 +126,9 @@ lemmas schedaction_related = sched_act_rct_related
 lemma kernelEntry_ex_abs[wp]:
   "\<lbrace>invs' and (\<lambda>s. e \<noteq> Interrupt \<longrightarrow> ct_running' s) and (ct_running' or ct_idle')
       and (\<lambda>s. vs_valid_duplicates' (ksPSpace s))
-      and (\<lambda>s. ksSchedulerAction s = ResumeCurrentThread) and ex_abs (einvs)\<rbrace>
+      and (\<lambda>s. ksSchedulerAction s = ResumeCurrentThread)
+      and (\<lambda>s. 0 < ksDomainTime s) and valid_domain_list'
+      and ex_abs (einvs)\<rbrace>
    kernelEntry_if e tc
    \<lbrace>\<lambda>_. ex_abs (einvs)\<rbrace>"
   apply (rule hoare_pre)
@@ -121,9 +136,9 @@ lemma kernelEntry_ex_abs[wp]:
    apply (wp kernel_entry_if_invs kernel_entry_if_valid_sched)
   apply (clarsimp simp: ex_abs_def)
   apply (rule_tac x=sa in exI)
-  apply (fastforce simp: ct_running_related ct_idle_related schedaction_related
-                         active_from_running' active_from_running)
-  done
+  apply (clarsimp simp: domain_time_rel_eq domain_list_rel_eq)
+  by (fastforce simp: ct_running_related ct_idle_related schedaction_related
+                      active_from_running' active_from_running)
 
 definition
   kernelCall_H_if
@@ -374,7 +389,7 @@ lemma doUserOp_if_invs'[wp]:
   apply (wp device_update_invs' dmo_setExMonitor_wp' dmo_invs' | simp)+
          apply (clarsimp simp add: no_irq_modify user_memory_update_def)
          apply wpsimp
-        apply (wp doMachineOp_ct_running' select_wp)+
+        apply (wp select_wp)+
   apply (clarsimp simp: user_memory_update_def simpler_modify_def
                         restrict_map_def
                   split: option.splits)
@@ -627,25 +642,32 @@ definition
   "handlePreemption_if tc \<equiv> do
      irq \<leftarrow> doMachineOp (getActiveIRQ False);
      when (irq \<noteq> None) $ handleInterrupt (the irq);
+     stateAssert (\<lambda>s. (ksDomainTime s = 0 \<longrightarrow> ksSchedulerAction s = ChooseNewThread) \<and>
+                       valid_domain_list' s) [];
      return tc
    od"
 
 crunch (empty_fail) empty_fail: handlePreemption_if
 
 lemma handle_preemption_if_corres:
- "corres (=) (einvs)
-   (invs')
-   (handle_preemption_if tc) (handlePreemption_if tc)"
+ "corres (=)
+         (einvs and valid_domain_list and (\<lambda>s. 0 < domain_time s))
+         (invs')
+         (handle_preemption_if tc) (handlePreemption_if tc)"
   apply (simp add: handlePreemption_if_def handle_preemption_if_def)
   apply (rule corres_guard_imp)
     apply (rule corres_split[where r'="(=)"])
        apply (rule corres_split[where r'="dc"])
-          apply simp
+          apply (rule corres_stateAssert_assume_stronger[where Q=\<top> and
+                        P="\<lambda>s. valid_domain_list s \<and>
+                               (domain_time s = 0 \<longrightarrow> scheduler_action s = choose_new_thread)"])
+           apply simp
+          apply (clarsimp simp: state_relation_def)
          apply (rule corres_when)
           apply simp
          apply simp
          apply (rule handle_interrupt_corres)
-        apply (rule hoare_post_taut[where P=\<top>])+
+        apply (wp handle_interrupt_valid_domain_time)+
       apply (rule dmo_getActiveIRQ_corres)
      apply (rule dmo_getActiveIRQ_wp)
     apply (rule dmo'_getActiveIRQ_wp)
@@ -657,7 +679,7 @@ lemma handle_preemption_if_corres:
 lemma handlePreemption_invs'[wp]:
   "\<lbrace>invs'\<rbrace> handlePreemption_if tc \<lbrace>\<lambda>_. invs'\<rbrace>"
   apply (simp add: handlePreemption_if_def)
-  apply (wp dmo'_getActiveIRQ_wp)
+  apply (wp dmo'_getActiveIRQ_wp hoare_drop_imps)
   apply clarsimp
   done
 
@@ -665,17 +687,19 @@ lemma handlePreemption_if_valid_duplicates[wp]:
   "\<lbrace>\<lambda>s. vs_valid_duplicates' (ksPSpace s)\<rbrace> handlePreemption_if tc
   \<lbrace>\<lambda>_ s. vs_valid_duplicates' (ksPSpace s)\<rbrace>"
   apply (simp add: handlePreemption_if_def)
-  apply (wp dmo'_getActiveIRQ_wp)
+  apply (wp dmo'_getActiveIRQ_wp hoare_drop_imps)
   apply clarsimp
   done
 
 lemma handlePreemption_ex_abs[wp]:
-  "\<lbrace>invs' and ex_abs (einvs)\<rbrace> handlePreemption_if tc \<lbrace>\<lambda>_. ex_abs (einvs)\<rbrace>"
+  "\<lbrace>invs' and ex_abs (einvs) and valid_domain_list' and (\<lambda>s. 0 < ksDomainTime s)\<rbrace>
+   handlePreemption_if tc
+   \<lbrace>\<lambda>_. ex_abs (einvs)\<rbrace>"
   apply (rule hoare_pre)
    apply (rule corres_ex_abs_lift[OF handle_preemption_if_corres])
    apply (wp handle_preemption_if_invs)
-  apply (auto simp: ex_abs_def non_kernel_IRQs_def)
-   done
+  apply (auto simp: ex_abs_def non_kernel_IRQs_def domain_list_rel_eq domain_time_rel_eq)
+  done
 
 lemma handle_preemption_if_valid_domain_time:
   "\<lbrace>\<lambda>s. 0 < domain_time s \<rbrace>
@@ -699,6 +723,7 @@ definition
   "schedule'_if tc \<equiv> do
      schedule;
      activateThread;
+     stateAssert (\<lambda>s. 0 < ksDomainTime s \<and> valid_domain_list' s) [];
      return tc
    od"
 
@@ -706,25 +731,30 @@ crunch (empty_fail) empty_fail: schedule'_if
 
 
 lemma schedule_if_corres:
- "corres (=) (invs and valid_sched and valid_list)
-   (invs')
-   (schedule_if tc) (schedule'_if tc)"
+ "corres (=)
+         (invs and valid_sched and valid_list and valid_domain_list and
+          (\<lambda>s. domain_time s = 0 \<longrightarrow> scheduler_action s = choose_new_thread))
+         (invs')
+         (schedule_if tc) (schedule'_if tc)"
   apply (simp add: schedule_if_def schedule'_if_def)
   apply (rule corres_guard_imp)
     apply (rule corres_split[where r'="dc"])
        apply (rule corres_split[where r'="dc"])
-          apply simp
+          apply (rule corres_stateAssert_assume_stronger[where Q=\<top> and
+                        P="\<lambda>s. valid_domain_list s \<and> 0 < domain_time s"])
+           apply simp
+          apply (clarsimp simp: state_relation_def)
          apply (rule activate_corres)
-        apply (rule hoare_post_taut[where P=\<top>])+
+        apply wp+
       apply (rule schedule_corres)
-     apply (wp schedule_invs')+
+     apply (wp schedule_invs' schedule_domain_time_left)+
    apply clarsimp+
   done
 
 lemma schedule_if'_invs'_post:
   "\<lbrace>invs'\<rbrace> schedule'_if tc \<lbrace>\<lambda>_. invs' and (ct_running' or ct_idle')\<rbrace>"
   apply (simp add: schedule'_if_def)
-  apply (wp activate_invs' schedule_invs' schedule_sch_act_simple | simp)+
+  apply (wp activate_invs' schedule_invs' schedule_sch_act_simple hoare_drop_imps | simp)+
   done
 
 lemma schedule_if'_invs'[wp]:
@@ -743,7 +773,7 @@ lemma schedule_if'_ct_running_or_idle[wp]:
 lemma schedule_if'_rct[wp]:
   "\<lbrace>invs'\<rbrace> schedule'_if tc \<lbrace>\<lambda>r s. ksSchedulerAction s = ResumeCurrentThread\<rbrace>"
   apply (simp add: schedule'_if_def)
-  apply (wp activate_sch_act schedule_sch)
+  apply (wp activate_sch_act schedule_sch hoare_drop_imps)
   done
 
 
@@ -751,7 +781,7 @@ lemma scheduler_if'_valid_duplicates[wp]:
   "\<lbrace>invs' and (\<lambda>s. vs_valid_duplicates' (ksPSpace s))\<rbrace> schedule'_if tc
   \<lbrace>\<lambda>_ s. vs_valid_duplicates' (ksPSpace s)\<rbrace>"
   apply (simp add: schedule'_if_def)
-  apply (wp | simp)+
+  apply (wp hoare_drop_imps | simp)+
   done
 
 lemma schedule_if_domain_time_left:
@@ -768,12 +798,22 @@ lemma schedule_if_domain_time_left:
   apply (auto split: if_split)
   done
 
+lemma sched_act_relation_ChooseNewThread[simp]:
+  "sched_act_relation sca ChooseNewThread = (sca = choose_new_thread)"
+  by (cases sca; simp)
+
 lemma scheduler'_if_ex_abs[wp]:
-  "\<lbrace>invs' and ex_abs (einvs)\<rbrace> schedule'_if tc \<lbrace>\<lambda>_. ex_abs (einvs)\<rbrace>"
+  "\<lbrace>invs' and ex_abs (einvs) and valid_domain_list' and
+    (\<lambda>s. ksDomainTime s = 0 \<longrightarrow> ksSchedulerAction s = ChooseNewThread)\<rbrace>
+   schedule'_if tc
+   \<lbrace>\<lambda>_. ex_abs (einvs)\<rbrace>"
   apply (rule hoare_pre)
    apply (rule corres_ex_abs_lift[OF schedule_if_corres])
    apply wp
-  apply (auto simp: ex_abs_def)
+  apply (clarsimp simp: ex_abs_def)
+  apply (rule exI, rule conjI, assumption)
+  apply (frule state_relation_schact)
+  apply (auto simp: domain_list_rel_eq domain_time_rel_eq)
   done
 
 definition
@@ -824,7 +864,8 @@ definition
 
 definition full_invs_if' where
   "full_invs_if' \<equiv>
-  {s. invs' (internal_state_if s) \<and> ex_abs (einvs) (internal_state_if s)
+  {s. invs' (internal_state_if s)
+      \<and> ex_abs (einvs) (internal_state_if s)
       \<and> vs_valid_duplicates' (ksPSpace (internal_state_if s))
       \<and> (snd s \<noteq> KernelSchedule True \<longrightarrow> ksDomainTime (internal_state_if s) > 0)
       \<and> (ksDomainTime (internal_state_if s) = 0
@@ -966,6 +1007,7 @@ lemma step_corresE:
     apply (rule d)
     apply simp+
     done
+
 end
 
 locale global_automaton_invs =
@@ -1008,8 +1050,8 @@ locale global_automaton_invs =
      apply (rule init_invs)
     apply (clarsimp simp: step_adt global_automaton_if_def)
     apply (elim disjE exE conjE,simp_all)
-apply (rule preservesE[OF kernel_call_invs])
-             apply (rule preservesE[OF kernel_call_invs],assumption+)
+             apply (rule preservesE[OF kernel_call_invs])
+                apply (rule preservesE[OF kernel_call_invs],assumption+)
             apply (rule preservesE[OF kernel_call_invs_sched],assumption+)
            apply (rule preservesE[OF handle_preemption_invs],assumption+)
           apply (rule preservesE[OF schedule_invs],assumption+)
@@ -1089,12 +1131,11 @@ lemmas preserves_lifts = preserves_lift_ret preserves_lift preserves_lift'
                          preserves_lift'' preserves_lift''' preserves'_lift
 
 
-
-
 defs step_restrict_def:
   "step_restrict \<equiv> \<lambda>s. s \<in> has_srel_state (lift_fst_rel (lift_snd_rel state_relation)) full_invs_if'"
 
 context begin interpretation Arch .
+
 lemma abstract_invs:
   "global_automaton_invs check_active_irq_A_if (do_user_op_A_if uop)
                          kernel_call_A_if kernel_handle_preemption_if
@@ -1156,6 +1197,7 @@ lemma abstract_invs:
     subgoal by (clarsimp cong: conj_cong | wp)+
    apply (fastforce simp: full_invs_if_def ADT_A_if_def step_restrict_def)+
   done
+
 end
 
 definition ADT_H_if where
@@ -1166,58 +1208,30 @@ definition ADT_H_if where
                               kernelCall_H_if handlePreemption_H_if
                               schedule'_H_if kernelExit_H_if)\<rparr>"
 
-crunch ksDomainTime_inv[wp]: doUserOp_if "(\<lambda>s. P (ksDomainTime s))"
+crunches doUserOp_if, checkActiveIRQ_if
+  for ksDomainTime_inv[wp]: "\<lambda>s. P (ksDomainTime s)"
+  and ksDomSchedule_inv[wp]: "\<lambda>s. P (ksDomSchedule s)"
   (wp: select_wp)
-
-crunch ksDomSchedule_inv[wp]: doUserOp_if "(\<lambda>s. P (ksDomSchedule s))"
-  (wp: select_wp)
-
-crunch ksDomainTime_inv[wp]: checkActiveIRQ_if "\<lambda>s. P (ksDomainTime s)"
-
-crunch ksDomSchedule_inv[wp]:
-  kernelEntry_if, handlePreemption_if, checkActiveIRQ_if, schedule'_if
-  "\<lambda>s. P (ksDomSchedule s)"
-
-lemma kernelEntry_if_ksDomainTime_inv:
-  "\<lbrace> K (e \<noteq> Interrupt) and (\<lambda>s. P (ksDomainTime s)) \<rbrace>
-   kernelEntry_if e tc
-   \<lbrace>\<lambda>_ s. P (ksDomainTime s) \<rbrace>"
-   unfolding kernelEntry_if_def
-   by (wp handleEvent_ksDomainTime_inv) simp
 
 lemma kernelEntry_if_valid_domain_time:
-  "\<lbrace>\<lambda>s. 0 < ksDomainTime s \<rbrace>
+  "e \<noteq> Interrupt \<Longrightarrow>
+   \<lbrace>\<top>\<rbrace> kernelEntry_if e tc \<lbrace>\<lambda>_ s. 0 < ksDomainTime s \<and> valid_domain_list' s\<rbrace>"
+
+  "\<lbrace>\<top>\<rbrace>
    kernelEntry_if Interrupt tc
-   \<lbrace>\<lambda>_ s. ksDomainTime s = 0 \<longrightarrow> ksSchedulerAction s = ChooseNewThread \<rbrace>"
-   unfolding kernelEntry_if_def
-  apply (clarsimp simp: handleEvent_def)
-  apply (rule hoare_pre)
-   apply (wp handleInterrupt_valid_domain_time | wpc | clarsimp)+
-       apply (rule hoare_false_imp) \<comment> \<open>debugPrint\<close>
-       apply (wp handleInterrupt_valid_domain_time hoare_vcg_all_lift hoare_drop_imps | simp)+
-  done
+   \<lbrace>\<lambda>_ s. (ksDomainTime s = 0 \<longrightarrow> ksSchedulerAction s = ChooseNewThread) \<and> valid_domain_list' s\<rbrace>"
+  unfolding kernelEntry_if_def by wpsimp+
 
 lemma handlePreemption_if_valid_domain_time:
-  "\<lbrace>\<lambda>s. 0 < ksDomainTime s \<rbrace>
+  "\<lbrace>\<top>\<rbrace>
    handlePreemption_if tc
-   \<lbrace>\<lambda>r s. ksDomainTime s = 0 \<longrightarrow> ksSchedulerAction s = ChooseNewThread \<rbrace>"
-   unfolding handlePreemption_if_def
-   apply (rule hoare_pre)
-   apply (wp handleInterrupt_valid_domain_time)
-   apply (rule_tac Q="\<lambda>_ s. 0 < ksDomainTime s" in hoare_post_imp, fastforce)
-   apply (wp, simp)
-   done
+   \<lbrace>\<lambda>_ s. (ksDomainTime s = 0 \<longrightarrow> ksSchedulerAction s = ChooseNewThread) \<and> valid_domain_list' s\<rbrace>"
+  unfolding handlePreemption_if_def by wpsimp
 
-lemma schedule'_if_domain_time_left:
-  "\<lbrace>\<lambda>s. valid_domain_list' s \<and> (ksDomainTime s = 0 \<longrightarrow> ksSchedulerAction s = ChooseNewThread) \<rbrace>
-   schedule'_if tc
-   \<lbrace>\<lambda>rv s. 0 < ksDomainTime s \<rbrace>"
-   unfolding schedule'_if_def
-   apply (rule hoare_pre)
-   apply wp
-   apply (rule hoare_post_imp[OF _ schedule_domain_time_left'])
-   apply clarsimp+
-   done
+lemma schedule'_if_valid_domain_time:
+  "\<lbrace>\<top>\<rbrace> schedule'_if tc \<lbrace>\<lambda>_ s. 0 < ksDomainTime s\<rbrace>"
+  "\<lbrace>\<top>\<rbrace> schedule'_if tc \<lbrace>\<lambda>_. valid_domain_list'\<rbrace>"
+  unfolding schedule'_if_def by wpsimp+
 
 lemma kernelEntry_if_no_preempt:
   "\<lbrace> \<top> \<rbrace> kernelEntry_if Interrupt ctx \<lbrace>\<lambda>(interrupt,_) _. interrupt = Inr () \<rbrace>"
@@ -1240,28 +1254,22 @@ lemma haskell_invs:
          apply simp
         apply (rule preserves_lifts)
         apply (simp add: full_invs_if'_def)
-        apply (wp kernelEntry_if_ksDomainTime_inv ; simp)
+        apply (wp kernelEntry_if_valid_domain_time; simp)
 
      subgoal for e
        apply (rule preserves_lifts, simp add: full_invs_if'_def)
        apply wp
-          apply (case_tac "e = Interrupt")
-           apply clarsimp
-           apply (wp kernelEntry_if_valid_domain_time ; simp)
-          apply clarsimp
-         apply (wp kernelEntry_if_ksDomainTime_inv ; simp)
+          apply (case_tac "e = Interrupt"; wpsimp wp: kernelEntry_if_valid_domain_time)
         apply fastforce+
        done
       subgoal
         apply (rule preserves_lifts, simp add: full_invs_if'_def)
-        apply (rule hoare_pre)
-        apply (wp handlePreemption_if_valid_domain_time ; simp)
+        apply (wp handlePreemption_if_valid_domain_time)
         apply fastforce
         done
      subgoal
        apply (rule preserves_lifts, simp add: full_invs_if'_def)
-       apply (rule hoare_pre)
-       apply (wp schedule'_if_domain_time_left)
+       apply (wp schedule'_if_valid_domain_time)
        apply fastforce
        done
     subgoal by (rule preserves_lifts, simp add: full_invs_if'_def)
