proof/crefine/ARM_HYP/Refine_C.thy
@@ -55,6 +55,7 @@ lemma handleInterruptEntry_ccorres:
      apply (simp add: irqInvalid_def ucast_helper_simps_32)
      apply (rule ccorres_symb_exec_r)
        apply (ctac (no_vcg) add: schedule_ccorres)
+        apply (rule ccorres_stateAssert_after)
         apply (rule ccorres_add_return2)
         apply (ctac (no_vcg) add: activateThread_ccorres)
          apply (rule_tac P=\<top> and P'=UNIV in ccorres_from_vcg_throws)
@@ -70,6 +71,7 @@ lemma handleInterruptEntry_ccorres:
     apply (ctac (no_vcg) add: handleInterrupt_ccorres)
      apply (rule ccorres_add_return, ctac (no_vcg) add: Arch_finaliseInterrupt_ccorres)
       apply (ctac (no_vcg) add: schedule_ccorres)
+       apply (rule ccorres_stateAssert_after)
        apply (rule ccorres_add_return2)
        apply (ctac (no_vcg) add: activateThread_ccorres)
         apply (rule_tac P=\<top> and P'=UNIV in ccorres_from_vcg_throws)
@@ -101,6 +103,7 @@ lemma handleUnknownSyscall_ccorres:
      apply (rule ccorres_pre_getCurThread)
      apply (ctac (no_vcg) add: handleFault_ccorres)
       apply (ctac (no_vcg) add: schedule_ccorres)
+       apply (rule ccorres_stateAssert_after)
        apply (rule ccorres_add_return2)
        apply (ctac (no_vcg) add: activateThread_ccorres)
         apply (rule_tac P=\<top> and P'=UNIV in ccorres_from_vcg_throws)
@@ -159,6 +162,7 @@ lemma handleVMFaultEvent_ccorres:
       apply ceqv
      apply clarsimp
      apply (ctac (no_vcg) add: schedule_ccorres)
+      apply (rule ccorres_stateAssert_after)
       apply (rule ccorres_add_return2)
       apply (ctac (no_vcg) add: activateThread_ccorres)
        apply (rule_tac P=\<top> and P'=UNIV in ccorres_from_vcg_throws)
@@ -189,6 +193,7 @@ lemma handleUserLevelFault_ccorres:
      apply (rule ccorres_pre_getCurThread)
      apply (ctac (no_vcg) add: handleFault_ccorres)
       apply (ctac (no_vcg) add: schedule_ccorres)
+       apply (rule ccorres_stateAssert_after)
        apply (rule ccorres_add_return2)
        apply (ctac (no_vcg) add: activateThread_ccorres)
         apply (rule_tac P=\<top> and P'=UNIV in ccorres_from_vcg_throws)
@@ -412,6 +417,7 @@ lemma handleSyscall_ccorres:
       \<comment> \<open>rest of body\<close>
       apply ceqv
      apply (ctac (no_vcg) add: schedule_ccorres)
+      apply (rule ccorres_stateAssert_after)
       apply (rule ccorres_add_return2)
       apply (ctac (no_vcg) add: activateThread_ccorres)
        apply (rule_tac P=\<top> and P'=UNIV in ccorres_from_vcg_throws)
@@ -498,10 +504,10 @@ definition
   "all_invs' e \<equiv> \<lambda>s'. \<exists>s :: det_state.
     (s,s') \<in> state_relation \<and>
     (einvs s \<and> (e \<noteq> Interrupt \<longrightarrow> ct_running s) \<and> (ct_running s \<or> ct_idle s) \<and>
-      scheduler_action s = resume_cur_thread \<and> domain_time s \<noteq> 0) \<and>
+      scheduler_action s = resume_cur_thread \<and> 0 < domain_time s \<and> valid_domain_list s) \<and>
     (invs' s' \<and> vs_valid_duplicates' (ksPSpace s') \<and>
-      (e \<noteq> Interrupt \<longrightarrow> ct_running' s') \<and> (ct_running' s' \<or> ct_idle' s') \<and>
-      ksSchedulerAction s' = ResumeCurrentThread  \<and> ksDomainTime s' \<noteq> 0)"
+      (e \<noteq> Interrupt \<longrightarrow> ct_running' s') \<and> (ct_running' s' \<or> ct_idle' s') \<and> ksDomainTime s' \<noteq> 0 \<and>
+      ksSchedulerAction s' = ResumeCurrentThread)"
 
 lemma no_fail_callKernel:
   "no_fail (all_invs' e) (callKernel e)"
@@ -525,12 +531,16 @@ lemma handleVCPUFault_ccorres:
    apply (rule ccorres_pre_getCurThread, rename_tac curThread)
    (* armv_handleVCPUFault returns false on this platform, doing nothing else *)
    apply (rule ccorres_symb_exec_r)
-   apply (rule ccorres_cond_false_seq, simp)
-   apply (rule ccorres_symb_exec_r)
-     apply (ctac (no_vcg) add: handleFault_ccorres)
-      apply (ctac (no_vcg) add: schedule_ccorres)
-       apply (ctac (no_vcg) add: activateThread_ccorres[simplified dc_def])
-      apply (wp schedule_sch_act_wf schedule_invs'|strengthen invs_queues invs_valid_objs')+
+     apply (rule ccorres_cond_false_seq, simp)
+     apply (rule ccorres_symb_exec_r)
+       apply (ctac (no_vcg) add: handleFault_ccorres)
+        apply (ctac (no_vcg) add: schedule_ccorres)
+         apply (rule ccorres_stateAssert_after)
+         apply (rule ccorres_guard_imp)
+           apply (ctac (no_vcg) add: activateThread_ccorres[simplified dc_def])
+          apply (clarsimp, assumption)
+         apply assumption
+        apply (wp schedule_sch_act_wf schedule_invs'|strengthen invs_queues invs_valid_objs')+
       apply vcg
      apply (clarsimp, rule conseqPre, vcg)
      apply clarsimp
